cedar-lean/Cedar/Thm/Validation/Typechecker/BinaryApp/GetTag.lean
@@ -94,28 +94,34 @@ theorem type_of_getTag_is_sound {x₁ x₂ : Expr} {c₁ c₂ : Capabilities} {e
   simp only [hf₁, Except.bind_ok, Except.bind_err, false_implies, Except.error.injEq, or_self, or_false, true_and,
     type_is_inhabited, and_self, reduceCtorEq]
   rw [Map.findOrErr_ok_iff_find?_some] at hf₁
-  replace ⟨entry, hf₂, _, _, _, h₂⟩  := h₂.right.left uid d hf₁
-  simp only [InstanceOfEntityTags] at h₂
-  simp [EntitySchema.tags?, Option.map_eq_some_iff] at ht
-  replace ⟨_, ht₁, ht₂⟩ := ht
-  simp only [hf₂, Option.some.injEq] at ht₁
-  subst ht₁
-  simp only [EntitySchemaEntry.tags?] at h₂ ht₂
-  split at ht₂
-  simp only [ht₂] at h₂
-  have hf₃ := Map.findOrErr_returns d.tags s Error.tagDoesNotExist
-  rcases hf₃ with ⟨v, hf₃⟩ | hf₃ <;>
-  simp only [hf₃, false_implies, Except.error.injEq, or_self, false_and, exists_const, and_false,
-    Except.ok.injEq, false_or, exists_eq_left', reduceCtorEq]
-  · simp only [htx, TypedExpr.typeOf, ← List.empty_eq, empty_capabilities_invariant request entities, implies_true, true_and, reduceCtorEq]
-    apply h₂
-    exact Map.findOrErr_ok_implies_in_values hf₃
-  · replace h₁ := h₁.right x₁ x₂ hc₁
-    simp only [EvaluatesTo, evaluate, ih₁, ih₂, apply₂, hasTag, Except.bind_ok, Except.ok.injEq,
-      Value.prim.injEq, Prim.bool.injEq, false_or, reduceCtorEq] at h₁
-    simp only [Entities.tagsOrEmpty, hf₁, Map.contains_iff_some_find?] at h₁
-    replace ⟨_, h₁⟩ := h₁
-    simp only [Map.findOrErr_err_iff_find?_none, h₁, reduceCtorEq] at hf₃
-  · cases ht₂
+  cases h₂.right.left uid d hf₁ with
+  | inl h =>
+    replace ⟨entry, hf₂, _, _, _, h₂⟩ := h
+    simp only [InstanceOfEntityTags] at h₂
+    simp [EntitySchema.tags?, Option.map_eq_some_iff] at ht
+    replace ⟨_, ht₁, ht₂⟩ := ht
+    simp only [hf₂, Option.some.injEq] at ht₁
+    subst ht₁
+    simp only [EntitySchemaEntry.tags?] at h₂ ht₂
+    split at ht₂
+    simp only [ht₂] at h₂
+    have hf₃ := Map.findOrErr_returns d.tags s Error.tagDoesNotExist
+    rcases hf₃ with ⟨v, hf₃⟩ | hf₃ <;>
+    simp only [hf₃, false_implies, Except.error.injEq, or_self, false_and, exists_const, and_false,
+      Except.ok.injEq, false_or, exists_eq_left', reduceCtorEq]
+    · simp only [htx, TypedExpr.typeOf, ← List.empty_eq, empty_capabilities_invariant request entities, implies_true, true_and, reduceCtorEq]
+      apply h₂
+      exact Map.findOrErr_ok_implies_in_values hf₃
+    · replace h₁ := h₁.right x₁ x₂ hc₁
+      simp only [EvaluatesTo, evaluate, ih₁, ih₂, apply₂, hasTag, Except.bind_ok, Except.ok.injEq,
+        Value.prim.injEq, Prim.bool.injEq, false_or, reduceCtorEq] at h₁
+      simp only [Entities.tagsOrEmpty, hf₁, Map.contains_iff_some_find?] at h₁
+      replace ⟨_, h₁⟩ := h₁
+      simp only [Map.findOrErr_err_iff_find?_none, h₁, reduceCtorEq] at hf₃
+    · cases ht₂
+  | inr h =>
+    replace ⟨_, _, h₂, _, _⟩ := h
+    simp only [EntitySchema.tags?, h₂, Option.map] at ht
+    contradiction
 
 end Cedar.Thm
