cedar-lean/Cedar/Validation/RequestEntityValidator.lean
@@ -99,7 +99,7 @@ For every entity in the store,
    in the type store.
 4. The entity's tags' types are consistent with the tags information in the type store.
 -/
-def instanceOfEntitySchema (entities : Entities) (ets : EntitySchema) : EntityValidationResult :=
+def instanceOfEntitySchema (entities : Entities) (ets : EntitySchema) (as : ActionSchema) : EntityValidationResult :=
   entities.toList.forM λ (uid, data) => instanceOfEntityData uid data
 where
   instanceOfEntityTags (data : EntityData) (entry : EntitySchemaEntry) : Bool :=
@@ -119,7 +119,14 @@ where
           else .error (.typeError s!"entity ancestors inconsistent with type store")
         else .error (.typeError "entity attributes do not match type store")
       else .error (.typeError s!"invalid entity uid: {uid}")
-    | _ => .error (.typeError "entity type not defined in type store")
+    | _ =>
+      match as.find? uid with
+      | .some _ =>
+        if data.attrs == Map.empty then
+          if data.tags == Map.empty then .ok ()
+          else .error (.typeError s!"action entitiy {uid} cannot have tags")
+        else .error (.typeError s!"action entitiy {uid} cannot have attributes")
+      | _ => .error (.typeError "entity type not defined in type store")
 
 /--
 For every action in the entity store, the action's ancestors are consistent
@@ -143,7 +150,7 @@ def validateRequest (schema : Schema) (request : Request) : RequestValidationRes
   else .error (.typeError "request could not be validated in any environment")
 
 def entitiesMatchEnvironment (env : Environment) (entities : Entities) : EntityValidationResult :=
-  instanceOfEntitySchema entities env.ets >>= λ _ => instanceOfActionSchema entities env.acts
+  instanceOfEntitySchema entities env.ets env.acts >>= λ _ => instanceOfActionSchema entities env.acts
 
 def actionSchemaEntryToEntityData (ase : ActionSchemaEntry) : EntityData := {
   ancestors := ase.ancestors,
